update dexp_size

proof/iu_system/decl/prop_typing.v
@@ -305,18 +305,24 @@ Definition dmode_size (mode : d_typing_mode) : nat :=
   end.
 
 
-Fixpoint dexp_size (e:dexp) : nat :=
-  match e with 
-  | dexp_unit => 1
-  | dexp_top => 1
-  | dexp_var_f _ => 1
-  | dexp_var_b _ => 1
-  | dexp_abs e1 => 1 + dexp_size e1
-  | dexp_app e1 e2 => dexp_size e1 + dexp_size e2 
-  | dexp_anno e1 _ => 1 + dexp_size e1
-  | dexp_tapp e1 _ => 1 + dexp_size e1
-  | dexp_tabs (dbody_anno e1 T) => 2 + dexp_size e1
-  end.
+Fixpoint 
+  dexp_size (e:dexp) : nat :=
+    match e with 
+    | dexp_unit => 1
+    | dexp_top => 1
+    | dexp_var_f _ => 1
+    | dexp_var_b _ => 1
+    | dexp_abs e1 => 1 + dexp_size e1
+    | dexp_app e1 e2 => dexp_size e1 + dexp_size e2 
+    | dexp_anno e1 _ => 1 + dexp_size e1
+    | dexp_tapp e1 _ => 1 + dexp_size e1
+    | dexp_tabs b => 1 + d_body_size b  
+    end with 
+  d_body_size (b:dbody) :=
+    match b with 
+    | dbody_anno e T => 1 + dexp_size e
+    end
+  .
 
 
 Fixpoint dtyp_size (T:dtyp) : nat :=
@@ -429,7 +435,28 @@ Admitted.
 
 Hint Extern 1 (_ < _) => lia : typing.
 Hint Extern 1 (_ ⊢ _) => eapply d_subenv_wf_typ; eauto : typing.
- 
+
+
+Lemma d_exp_size_open_var_rec : forall e x n, 
+  dexp_size e = dexp_size (open_dexp_wrt_dexp_rec n (dexp_var_f x) e)
+with d_body_size_open_var_rec: forall b x n,
+  d_body_size b = d_body_size (open_dbody_wrt_dexp_rec n (dexp_var_f x) b).
+Proof.
+  - intros. generalize dependent n. induction e; simpl; auto.
+    + intros. destruct (lt_eq_lt_dec n n0).
+      * destruct s; auto.
+      * auto.
+  - intros. generalize dependent n. induction b; simpl; auto.
+Qed.
+
+
+Lemma d_exp_size_open_var: forall e x,
+  dexp_size e = dexp_size (open_dexp_wrt_dexp e (dexp_var_f x)).
+Proof.
+  intros. unfold open_dexp_wrt_dexp.
+  apply d_exp_size_open_var_rec.
+Qed.
+
 Theorem d_chk_inf_subsumption : forall n1 n2 n3 E E' e T1 mode,
   dexp_size e < n1 ->
   dmode_size mode < n2 ->
@@ -493,9 +520,9 @@ Proof with auto with typing.
            inst_cofinites_with x.
            simpl in H.
            refine (IHn1 _ _ _ _ _ _ _ _ _ _ H2 _ _ _); eauto...
-           admit. (* exp_size  ** *)
+           rewrite <- d_exp_size_open_var. lia.
       (* \x. e <= T1 -> T2 *)
-      * intros. 
+      * intros. simpl in H.
         assert (d_wft_ord S1). admit. (* trivial * *)
         induction H6.
         -- dependent destruction H5.
@@ -507,7 +534,7 @@ Proof with auto with typing.
            ++ inst_cofinites_for d_typing_chkabs.
               admit. intros. inst_cofinites_with x.
               refine (IHn1 _ _ _ _ _ _ _ _ _ _ H3 _ _ _); eauto...
-              admit. (* exp_size ** *)
+              rewrite <- d_exp_size_open_var. lia.
               admit. (* sub_weakening *)
            ++ inversion H6.
            ++ inversion H7.
